\documentclass{article}
\usepackage{math_template}

\author{Jonathan Kasongo}
\title{Croatia IMO Team Selection Test 2009 --- P1/4}

\begin{document}
\maketitle

\begin{problem}{Croatia IMO Team Selection Test 2009 --- P1/4}
Find all real numbers $x, y, z$ such that the following two equations are satisfied:
$$
\begin{aligned}
3\left(x^2+y^2+z^2\right) & =1 \\
x^2 y^2+y^2 z^2+z^2 x^2 & =x y z(x+y+z)^3
\end{aligned}
$$
\end{problem}

\begin{solution}{Solution}
\textit{Lemma: $xy + yz + zx = \frac{1}{2} (x+y+z)^2 - \frac{1}{6}$}.\\

\textit{Proof:} Use the first equation to see that $(x^2+y^2+z^2) =
(x+y+z)^2 - 2(xy+yz+zx) = \frac{1}{3}$ and so
$xy + yz + zx = \frac{1}{2} (x+y+z)^2 - \frac{1}{6}$ as desired.\\

Now using our lemma observe that,

\[
\begin{aligned}
(x+y+z)^3 &= x^3 + y^3 + z^3 + 3(x+y+z)(xy+yz+zx) - 3xyz \\
&= x^3 + y^3 + z^3 + 3(x+y+z)\left(\frac{1}{2} (x+y+z)^2 - \frac{1}{6}\right) - 3xyz \\
&= x^3 + y^3 + z^3 + \frac{3}{2}(x+y+z)^3 - \frac{1}{2} (x+y+z) - 3xyz\\
\frac{1}{2}(x+y+z)^3 &= \frac{1}{2} (x+y+z) + 3xyz - (x^3 + y^3 + z^3)\\
\end{aligned}
\]

Now the second equation asserts that
$\sum_{\text{sym}} x^2 y^2 = xyz((x+y+z) + 6xyz - 2(x^3+y^3+z^3))$ so

$$
2xyz(x^3 + y^3 + z^3) + (x^2 y^2 + y^2 z^2 + z^2 x^2) =
6(xyz)^2 + xyz(x+y+z)
$$

If we have $xyz=0$ then the equation becomes
$(x^2 y^2 + y^2 z^2 + z^2 x^2) = 0$ and so $xy = yz = zx = 0$ and
at least 2 of $x,y,z$ must be 0. Suppose without loss of generality that
$x=y=0$, then we just need $3z^2 = 1 \iff z = \pm \frac{1}{\sqrt{3}}$.
So $(x,y,z)=\left(0,0,\pm \frac{1}{\sqrt{3}}\right)$ is a solution up to it's 6 permutations.\\


Now assuming that $x,y,z > 0$  and $xyz > 0$, we can say
by AM-GM, $2xyz(x^3 + y^3 + z^3) \geq 6(xyz)^2$ and by Muirhead's
inequality, $\sum_{\text{sym}} x^2 y^2 z^0 = (x^2 y^2 + y^2 z^2 + z^2 x^2)
\geq xyz(x+y+z) = \sum_{\text{sym}} x^2 yz$ since $(2,2,0)\succ (2,1,1)$.
But that means we must have the equality case in both of these
inequalities. AM-GM reaches equality exactly when $x=y=z$, so we must
have $9x^2 = 1 \iff x = \pm \frac{1}{3}$ and $3x^4 = 27x^6 \iff
3x^4(9x^2 - 1) = 3x^4 (3x-1)(3x+1) = 0 \iff x = \pm \frac{1}{3} \ \text{or} \ 0$
so the only solutions here are $x=y=z=\left(\frac{1}{3}, \frac{1}{3},\frac{1}{3}\right)$.
Now since we assumed that $x,y,z$ are positive we know that in fact each
one of $x,y,z$ could be $\pm \frac{1}{3}$. But it is straightforward to
check each case, we have up to permutations,
$(\frac{1}{3}, \frac{1}{3}, \frac{1}{3})$ which we know works.
$(\frac{1}{3}, \frac{1}{3}, -\frac{1}{3})$ but that makes the RHS of second
equation $<0$ whilst the LHS is $\geq 0$, so it's impossible.
$(\frac{1}{3}, -\frac{1}{3}, -\frac{1}{3})$ makes $x+y+z$ negative whilst
$xyz > 0$ so this is also impossible by the same reason as the last case.
$(-\frac{1}{3}, -\frac{1}{3}, -\frac{1}{3})$ which works since
$3 \cdot \frac{1}{81} = -\frac{1}{27} \cdot -1$
\end{solution}

\end{document}
