\documentclass{article}
\usepackage{math_template}

\author{Jonathan Kasongo}
\title{POTD 1254}

\begin{document}
\maketitle

\begin{problem}{POTD 1254}
If $a, b, c>0$ and $a+b+c=6$, show that
$$
\left(a+\frac{1}{b}\right)^2+\left(b+\frac{1}{c}\right)^2+\left(c+\frac{1}{a}\right)^2 \geq \frac{75}{4} .
$$
\end{problem}

\begin{solution}{Solution}
In this solution any summation terms $\sum$ are assumed to be cyclic over
$a,b,c$, that is for a function $f$, $\sum f(a,b,c) = f(a,b,c) + f(b,c,a) + f(c,a,b)$.
The inequality is symmetric so we may assume, without loss of generality,
that $a\geq b\geq c$. We start of by showing some useful inequalities.
Firstly using QM-AM, we get that $\frac{1}{3} (a+b+c) = 2 \leq
\sqrt{(a^2 + b^2 + c^2) / 3}$ and so $12 \leq a^2 + b^2 + c^2$. Using
the Re-arragement inequality on the sequences $a\geq b\geq c$ and
$\frac{1}{c} \geq \frac{1}{b} \geq \frac{1}{a}$ we can show that
$2\left(\frac{a}{b} + \frac{b}{c} + \frac{c}{a}\right) \geq
2\left(\frac{a}{a} + \frac{b}{b} + \frac{c}{c}\right)=6$.
We can now use these 2 results. Expand the LHS to get that
$\sum a^2 + 2\sum \frac{a}{b} + \sum \frac{1}{a^2} \geq
\frac{75}{4}$.
By our 2 results we can see that it suffices to show that
$\sum \frac{1}{a^2} \geq \frac{75}{4} - 12 - 6 = \frac{3}{4}$.
By AM-GM we know that $a+b+c=6\geq 3(abc)^{1/3} \iff 2\geq (abc)^{1/3}
\iff 8 \geq abc \iff \frac{1}{8} \leq \frac{1}{abc}$. Now by the
Re-arragement inequality on the sequence $\frac{1}{c} \geq \frac{1}{b} \geq
\frac{1}{a}$ and itself coupled with the fact that $a+b+c=6$ we know that
$\sum \frac{1}{a^2} \geq \sum
\frac{1}{ac} = \frac{1}{abc} (a+b+c) = \frac{6}{abc} \geq \frac{6}{8} =
\frac{3}{4}$ as desired. This finishes the problem. $\blacksquare$
\end{solution}

\end{document}
